finished append lemma for partially ordered sequences.

src/spec/Flutterbye.Seq.Ordered.fst
@@ -36,72 +36,38 @@ abstract val slice_lemma:
 let slice_lemma lte s =
    ()
 
-val tmp_lemma:
+val append_lemma_loop:
    lte:compare_t 'a{partial_order_p lte} ->
    s:seq 'a{ordered_p lte s} ->
    a: 'a ->
+   i:nat{0 < i && i <= length s} ->
    Lemma
-      (ensures 
-            (forall (x:nat{x < length s}). lte (index s x) a))
-let tmp_lemma lte s a =
-   admit ()
+      (requires 
+        (forall (x:nat{x < length s}). 
+            x >= length s - i ==> lte (index s x) a))
+      (ensures (forall (x:nat{x < length s}). lte (index s x) a))
+      (decreases (length s - i))
+let rec append_lemma_loop lte s a i =
+   if i < length s then
+      let a_i = index s (length s - 1 - i) in
+      // both of the following assertions are necessary to
+      // estabilsh the transitivity of a_i <= a_last <= a.
+      assert (lte a_i (index s (length s - 1)));
+      assert (lte a_i a);
+      append_lemma_loop lte s a (i + 1)
+   else
+      ()
 
-abstract val append_lemma_loop:
+abstract val append_lemma:
    lte:compare_t 'a{partial_order_p lte} ->
    s:seq 'a{ordered_p lte s} ->
    a: 'a ->
    Lemma
       (requires (length s = 0 || lte (index s (length s - 1)) a))
       (ensures (ordered_p lte (append s (create 1 a))))
-let append_lemma_loop lte s a =
-   if length s > 1 then
-      begin
-         tmp_lemma lte s a;
-         ()
-      end
-   else
+let append_lemma lte s a =
+   if length s = 0 then
       ()
-
-      (*
-abstract val append_lemma:
-   lte:compare_t 'a{partial_order_p lte} ->
-   s_1:seq 'a{ordered_p lte s_1} ->
-   s_2:seq 'a{ordered_p lte s_2} ->
-   Lemma
-      (*(requires (
-         // either `s_1` or `s_2` are of zero length
-         length s_1 = 0 || length s_2 = 0
-         // or the first element of `s_2` must not be less than the final element of `s_1`.
-         || lte (index s_1 (length s_1 - 1)) (index s_2 0)
-      ))*)
-      (ensures (ordered_p lte (append s_1 s_2)))
-let append_lemma lte s_1 s_2 =
-   if length s_1 > 0 && length s_2 > 0 then
-      begin
-         let s' = append s_1 s_2 in
-         assert
-            (forall (x:nat{x < length s_1}) (y:nat{y < length s_1}).
-               ((x <= y) <==> (lte (index s' x) (index s' y))));
-         assert
-            (forall (x:nat{x < length s_2}) (y:nat{y < length s_2}).
-               ((x <= y) <==> (lte (index s' (x + length s_1)) (index s' (y + length s_1)))));
-         assert (length s' = length s_1 + length s_2);
-         assert (length s_1 - 1 >= 0);
-         assert (lte (index s' (length s_1 - 1)) (index s' (length s_1)));
-         assert
-            (forall (x:nat{x <= length s_1}) (y:nat{y <= length s_1}).
-               ((x <= y) <==> (lte (index s' x) (index s' y))));
-         assert
-            (forall (x:nat{x < length s'}) (y:nat{y < length s'}).
-               ((x <= y) <==> (lte (index s' x) (index s' y))));
-         admit ()
-      end
    else
-      ()*)
+      append_lemma_loop lte s a 1
 
-      (*(requires (
-         // either `s_1` or `s_2` are of zero length
-         length s_1 = 0 || length s_2 = 0
-         // or the first element of `s_2` must not be less than the final element of `s_1`.
-         || lte (index s_1 (length s_1 - 1)) (index s_2 0)
-      ))*)
